ContractExamples/FStar/CallOption.fst
@@ -1,26 +1,40 @@
-module CallOption
+module ZenModule
 
 open Zen.Base
 open Zen.Types
 open Zen.Wallet
+open Zen.Cost
 
+module      V = Zen.Vector
+module    U64 = FStar.UInt64
 module Crypto = Zen.Crypto
 
-module U64 = FStar.UInt64
+let numeraire: hash = Zen.Util.hashFromBase64 "AAAAAAAAAAAAAAAAAAAAAAAAAAAAAAAAAAAAAAAAAAA="
 
-assume val numeraire: hash
 let price: U64.t = 100UL
-assume val ownerPubKey: Crypto.key
+//assume val ownerPubKey: Crypto.key
 
-assume val msgSig: signature
+//assume val msgSig: signature
 
+type command =
+  | Collateralize
+  | Buy
+  | Exercise
+  | Close
+  | Fail
+
+val parseCommand: opcode -> command
+let parseCommand  opcode = if opcode = 0uy then Collateralize
+                      else if opcode = 1uy then Buy
+                      else if opcode = 2uy then Exercise
+                      else if opcode = 3uy then Close else Fail
 
 type state = { tokensIssued : U64.t;
                collateral   : U64.t;
-               counter      : U64.t;
-               wallet       : wallet }
+               counter      : U64.t }
 
-//assume val isAuthenticated: inputMsg -> bool
+
+(*assume val isAuthenticated: inputMsg -> bool
 
 val isAuthenticated : inputMsg -> bool
 let isAuthenticated inputMsg =
@@ -39,37 +53,89 @@ let correctDataForm inputMsg =
 
 val isValid: inputMsg -> bool
 let isValid inputMsg = isAuthenticated inputMsg &&
-                       correctDataForm inputMsg
-
-assume val getState: inputMsg:inputMsg{isValid inputMsg} * wallet -> state
-
-val collateralize: state -> state
-let collateralize s = let open U64 in
-  let recieveAmount: U64.t = admit() in
-  { s with counter   =   s.counter +%^ 1UL;            // increment the counter
-           collateral=s.collateral +%^ recieveAmount }
+                       correctDataForm inputMsg*)
 
 
-val buy: inputMsg -> state -> option state
-let buy inputMsg state = let open U64 in
+
+val getOutputs: inputMsg ->
+  receiving : option output *
+  state     : option output
+let getOutputs { data = (| _, data |); utxo = utxo } = match data with
+  | Data2 _ _ (Outpoint receiving) (Optional _ state)
+    -> let state = match state with
+                    | Some (Outpoint o) -> utxo o
+                    | _ -> None in
+       utxo receiving, state
+  | _ -> None, None
+
+val getState: contractHash:hash -> output -> option state
+let getState contractHash = function
+  | { spend = { asset = asset; amount = collateral };
+      lock = ContractLock cHash _ (Data2 _ _ (UInt64 tokensIssued)
+                                             (UInt64 counter)) }
+     -> if contractHash <> cHash || asset <> numeraire
+        then None
+        else Some @ { tokensIssued = tokensIssued;
+                      collateral   = collateral;
+                      counter      = counter }
+  | _ -> None
+
+val makeStateOutput: contractHash:hash -> state -> output
+let makeStateOutput contractHash state =
+  let data = Data2 _ _
+                   (UInt64 state.tokensIssued)
+                   (UInt64 state.counter) in
+  {  spend = { asset = numeraire; amount = state.collateral };
+     lock = ContractLock contractHash _ data }
+
+
+val makeTx:
+     contractHash:hash
+  -> #l:nat -> V.t outpoint l
+  -> state
+  -> option output
+  -> transactionSkeleton
+let makeTx contractHash #_ outpoints state output =
+  let stateOutput = V.VCons (makeStateOutput contractHash state) V.VNil in
+  match output with
+    | None        -> Tx outpoints stateOutput None
+    | Some output -> Tx outpoints (V.VCons output stateOutput) None
+
+val collateralize:
+     option state
+  -> receiving: output
+  -> option state * option output
+let collateralize s receiving = let open U64 in
+  if receiving.spend.asset <> numeraire then None, None
+  else
+    let receiveAmount = receiving.spend.amount in
+    let state = match s with
+      | None -> { counter = 1UL; collateral = receiveAmount; tokensIssued = 0UL }
+      | Some s -> { s with counter    = s.counter +%^ 1UL;            // increment the counter
+                           collateral = s.collateral +%^ receiveAmount } in
+
+    Some state, None
+
+//assume val buy: inputMsg -> state -> option state
+(*let buy inputMsg state = let open U64 in
   match inputMsg.data with
   | (| _, Data2 _ _ (Hash senderPKHash) (Hash returnPKHash) |) ->
-    let recieveAmount   = getFundsFrom state.wallet numeraire senderPKHash in
-    let tokensPurchased = recieveAmount /^ price in
+    let receiveAmount   = getFundsFrom state.wallet numeraire senderPKHash in
+    let tokensPurchased = receiveAmount /^ price in
 
     let output = { lock=PKLock returnPKHash;
                    spend= { asset =inputMsg.contractHash;
                             amount=tokensPurchased } } in
 
     Some @ { state with wallet = state.wallet `addOutput` unsafe_coerce output;
-                        collateral   = state.collateral   +%^ recieveAmount;
+                        collateral   = state.collateral   +%^ receiveAmount;
                         tokensIssued = state.tokensIssued +%^ tokensPurchased }
-  | _ -> None
+  | _ -> None*)
 
-assume val exercise     : state -> state
+//assume val exercise     : state -> state
 
-val close: inputMsg -> state -> option state
-let close inputMsg state =
+//assume val close: inputMsg -> state -> option state
+(*let close inputMsg state =
   match inputMsg.data with
   | (| _, Hash returnPKHash |) ->
     let output = { lock=PKLock returnPKHash;
@@ -77,19 +143,25 @@ let close inputMsg state =
                             amount=state.wallet `getFunds` numeraire } } in
     Some @ { state with wallet = state.wallet `addOutput` output;
                         collateral = 0UL }
-  | _ -> None
+  | _ -> None*)
 
-val fail: 'a -> option state
-let fail _ = None
+val main: inputMsg -> cost (result transactionSkeleton) 0
+let main i = let open Zen.Option in
+   //TODO: Improve pattern match on machine integers.
+  //if not (isValid inputMsg) then fail inputMsg else
 
-val main: inputMsg * wallet -> option state
-let main (inputMsg, wallet) = //TODO: Improve pattern match on machine integers.
-  if not (isValid inputMsg) then fail inputMsg else
-  let cmd = inputMsg.cmd in
-  let action = if cmd = 0uy then collateralize >> Some
-          else if cmd = 1uy then buy inputMsg
-          else if cmd = 2uy then exercise >> Some
-          else if cmd = 3uy then close inputMsg
-                            else fail in
-  let state = getState (inputMsg, wallet) in
-  action state
+  let receiving, state = getOutputs i in
+  let state = state `bind` getState i.contractHash in
+
+  ret (match receiving with
+    | None -> Err "could not resolve 'receiving' outpoint"
+    | Some receiving ->
+      let state', output = match parseCommand i.cmd with
+        | Collateralize -> collateralize state receiving
+        | Buy
+        | Exercise
+        | Close
+        | Fail -> None, None in
+      match state' with
+        | None        -> Err "test"
+        | Some state' -> V (makeTx i.contractHash V.VNil state' output))
